dev2020/dsubsup_cc/coq.v
@@ -110,13 +110,13 @@ Proof.
   - apply IHctx_wf in H2. apply ty_wf_weaken. assumption. constructor. assumption. assumption.
 Qed.
 
-(* Lemma hcwf: forall {Gamma e T}, has_type Gamma e T -> ctx_wf Gamma *)
-(*     with *)
-(*     tcwf: forall {Gamma T}, ty_wf Gamma T -> ctx_wf Gamma. *)
-(* Proof. *)
-(*   - intros. induction H; eauto. *)
-(*   - intros. induction H; eauto. *)
-(* Qed. *)
+Lemma hcwf: forall {Gamma e T}, has_type Gamma e T -> ctx_wf Gamma
+    with
+    tcwf: forall {Gamma T}, ty_wf Gamma T -> ctx_wf Gamma.
+Proof.
+  - intros. induction H; eauto.
+  - intros. induction H; eauto.
+Qed.
 
 Lemma extract1: forall Gamma T1 T2, ty_wf Gamma (TMem T1 T2) -> ty_wf Gamma T2.
 Proof.
@@ -143,9 +143,9 @@ Proof.
     generalize dependent Gamma. generalize dependent e. generalize dependent T1.
     induction T2; intros.
     (* TTop *)
-    -- simpl. constructor.
+    -- simpl. constructor. eapply hcwf. eauto.
     (* TBot *)
-    -- simpl. constructor.
+    -- simpl. constructor. eapply hcwf. eauto.
     (* TAll *)
     -- simpl in H. inversion H. subst. simpl. constructor.
        --- eapply IHT2_1; eauto.
@@ -172,7 +172,8 @@ Admitted. (*TODO: most of the cases are wrong, try avoiding eauto *)
 Lemma htwf: forall {Gamma e T}, has_type Gamma e T -> ty_wf Gamma T.
 Proof.
   intros. induction H; auto.
-  - apply wf_sel with (T1 := T1) (T2 := TTop); auto. constructor.
+  - eapply wf_lookup; eauto.
+  - apply wf_sel with (T1 := T1) (T2 := TTop); auto. constructor. eapply tcwf. eauto.
   - apply (extract1 _ _ _ IHhas_type2).
   - constructor; auto.
   - inversion IHhas_type1. subst. eapply ty_wf_open; eauto.
@@ -296,12 +297,14 @@ structural properties:
 
 Section Interp.
 
+  Polymorphic Definition TYPE =
+
   (* Polymorphic Fixpoint tctx {Gamma} (wf: D.ctx_wf Gamma): list Type (* ctx ???  *)    := *)
   (*   match wf with *)
   (*   | D.wf_empty => [] *)
   (*   | D.wf_cons Gamma T wf_Gamma_T wf_Gamma => (ttp wf_Gamma_T) :: (tctx wf_Gamma) *)
   (*   end *)
-  Polymorphic Fixpoint ttp {Gamma} {T} (ty_wf: D.ty_wf Gamma T): Type :=
+  Polymorphic Fixpoint ttp {Gamma} {T} (ty_wf: D.ty_wf Gamma T): { Gamma : tenv & venv Gamma -> Type}  :=
     match ty_wf with
     | D.wf_top _ =>
       TTop
